wp and twp example in intro of paper

theories/ub_logic/ub_examples.v
@@ -1,7 +1,147 @@
 From clutch.ub_logic Require Export ub_clutch.
 
+Section test.
+  Context `{!ub_clutchGS Σ}.
+
+  Definition φ v :iProp Σ:= (⌜v = #true⌝)%I.
+
+  Definition loop:val:=
+    rec: "loop" "x" := "loop" "x".
+  
+  Definition e' (n:expr) : expr :=
+    let: "k" := rand #1 in
+    if: n+"k" ≤ #2 then
+      #true
+    else
+      if: n+"k"=#3
+      then #false
+      else loop #().
+  
+  Definition e :expr :=
+    let: "n" := rand #3 in
+    if: "n"≤#1
+    then #true
+    else e' "n".
+
+  Lemma loop_lemma E (v:val) Φ:
+    ⊢ WP (loop v) @ E {{Φ}}.
+  Proof.
+    iLöb as "IH".
+    rewrite /loop.
+    by wp_pures.
+  Qed.
+  
+  Lemma twp_e'_two E:
+    ⊢ € (nnreal_half) -∗ WP (e' #2) @ E [{ φ }].
+  Proof.
+    iIntros "Herr".
+    rewrite /e'.
+    wp_apply (twp_rand_err_nat _ _ 1).
+    iSplitL.
+    - iApply (ec_spend_irrel with "[$]").
+      simpl. lra.
+    - iIntros (x) "%".
+      wp_pures.
+      pose proof (fin_to_nat_lt x).
+      destruct (fin_to_nat x); last lia.
+      case_bool_decide; last lia.
+      by wp_pures.
+  Qed.
+
+  Lemma wp_e'_two E:
+    ⊢ € (nnreal_half) -∗ WP (e' #2) @ E {{ φ }}.
+  Proof.
+    iIntros "Herr".
+    iApply ub_twp_ub_wp'.
+    by iApply twp_e'_two.
+  Qed.
+
+  Lemma twp_e'_three E:
+    ⊢ € (nnreal_one) -∗ WP (e' #3) @ E [{ φ }].
+  Proof.
+    iIntros "Herr".
+    iExFalso.
+    iApply ec_spend; last done.
+    simpl. lra.
+  Qed.
+
+  Lemma wp_e'_three E:
+    ⊢ € (nnreal_half) -∗ WP (e' #3) @ E {{ φ }}.
+  Proof.
+    iIntros "Herr".
+    rewrite /e'.
+    wp_apply (wp_rand_err_nat _ _ 0).
+    iSplitL.
+    - iApply (ec_spend_irrel with "[$]").
+      simpl. lra.
+    - iIntros (x) "%".
+      wp_pures.
+      pose proof (fin_to_nat_lt x).
+      destruct (fin_to_nat x); first lia.
+      assert (n=0) as -> by lia.
+      case_bool_decide; first lia.
+      wp_pures.
+      wp_apply loop_lemma.
+  Qed.
+  
+  Lemma twp_e E:
+    ⊢ € (nnreal_div (nnreal_nat 3) (nnreal_nat 8)) -∗
+    WP e @ E [{φ}].
+  Proof.
+    iIntros "Herr".
+    rewrite /e.
+    set (ε2 := λ n : fin (S 3), if (fin_to_nat n <? 2) then nnreal_zero else
+                      if (fin_to_nat n =? 2) then nnreal_half else nnreal_one)
+        .
+        wp_apply (twp_couple_rand_adv_comp1 _ _ _ _ ε2 with "[$]").
+        { rewrite SeriesC_finite_foldr. simpl. lra. }
+        iIntros (n) "Herr".
+        wp_pures. 
+        case_bool_decide; wp_pures; first done.
+        pose proof (fin_to_nat_lt n).
+        eassert (n=nat_to_fin (_:2<4) \/ n = nat_to_fin (_ :3<4)) as [-> | ->].
+        { Unshelve.
+          all: try lia.
+          simpl.
+          destruct (fin_to_nat n) as [|[|[|[|]]]] eqn:Hn; [lia|lia|left|right| lia].
+          - by repeat (inv_fin n; [done|intros n ?]).
+          - by repeat (inv_fin n; [done|intros n ?]).
+        }
+    - by wp_apply twp_e'_two.
+    - by wp_apply twp_e'_three.
+  Qed.
+
+  Lemma wp_e E:
+    ⊢ € (nnreal_div (nnreal_nat 1) (nnreal_nat 4)) -∗
+    WP e @ E {{φ}}.
+  Proof.
+    iIntros "Herr".
+    rewrite /e.
+    set (ε2 := λ n : fin (S 3), if (fin_to_nat n <? 2) then nnreal_zero else
+                      if (fin_to_nat n =? 2) then nnreal_half else nnreal_half)
+        .
+        wp_apply (wp_couple_rand_adv_comp1 _ _ _ _ ε2 with "[$]").
+        { rewrite SeriesC_finite_foldr. simpl. lra. }
+        iIntros (n) "Herr".
+        wp_pures. 
+        case_bool_decide; wp_pures; first done.
+        pose proof (fin_to_nat_lt n).
+        eassert (n=nat_to_fin (_:2<4) \/ n = nat_to_fin (_ :3<4)) as [-> | ->].
+        { Unshelve.
+          all: try lia.
+          simpl.
+          destruct (fin_to_nat n) as [|[|[|[|]]]] eqn:Hn; [lia|lia|left|right| lia].
+          - by repeat (inv_fin n; [done|intros n ?]).
+          - by repeat (inv_fin n; [done|intros n ?]).
+        }
+    - by wp_apply wp_e'_two.
+    - by wp_apply wp_e'_three.
+  Qed.
+    
+End test.
 
 Local Open Scope R.
+
 Context `{!ub_clutchGS Σ}.
 
 Definition foo N (m : nat) : expr :=
